DeBruijnSSA/BinSyntax/Rewrite/Region/Structural/Elgot.lean
@@ -1,4 +1,5 @@
-import DeBruijnSSA.BinSyntax.Rewrite.Region.Structural.Gloop
+import DeBruijnSSA.BinSyntax.Rewrite.Region.Structural.Letc
+import DeBruijnSSA.BinSyntax.Rewrite.Region.Structural.Sum
 import DeBruijnSSA.BinSyntax.Rewrite.Region.Compose.Elgot
 
 namespace BinSyntax
@@ -6,3 +7,18 @@ namespace BinSyntax
 variable [Φ: EffInstSet φ (Ty α) ε] [PartialOrder α] [SemilatticeSup ε] [OrderBot ε]
 
 namespace Region
+
+def Eqv.fixpoint_def' {A B : Ty α} {Γ : Ctx α ε} {L : LCtx α} (f : Eqv φ (⟨A, ⊥⟩::Γ) ((B.coprod A)::L))
+  : Eqv φ (⟨A, ⊥⟩::Γ) (B::L) := letc A nil (f.vwk1.lwk1 ;; left_exit)
+
+theorem Eqv.letc_to_vwk1 {Γ : Ctx α ε} {L : LCtx α} {A : Ty α} {β : Eqv φ ((B, ⊥)::Γ) (A::L)} {G}
+  : letc A β G = letc (B.prod A)
+    (ret Term.Eqv.split ;; _ ⋊ β)
+    ((ret Term.Eqv.split ⋉ _ ;; assoc ;; _ ⋊ (let2 (Term.Eqv.var 0 Ctx.Var.shead) G.vwk2)).vwk1)
+  := by
+  sorry
+
+theorem Eqv.letc_vwk1_den {Γ : Ctx α ε}
+  {A B : Ty α} {β : Eqv φ ((X, ⊥)::Γ) [A, B]} {G : Eqv φ ((A, ⊥)::Γ) [A, B]}
+  : letc A β G.vwk1 = β.packed_out ;; fixpoint (coprod (coprod zero inj_l) (G.packed_out ;; inj_r))
+  := sorry
